AST proof of 1D uniform random walk

theories/eris/examples/random_walk.v
@@ -1,9 +1,9 @@
+From clutch.eris Require Export adequacy total_adequacy.
 From clutch.eris Require Export eris error_rules.
-From clutch Require Export examples.approximate_samplers.approx_sampler_lib.
 From Coquelicot Require Import Series.
-Require Import Lra.
 
 Set Default Proof Using "Type*".
+
 
 Section uniform_random_walk.
 
@@ -17,7 +17,7 @@ Section uniform_random_walk.
     (rec: "f" "n" "α" :=
       if: "n" < #1
       then #()
-      else let: "x" := (rand ("α") #1) in
+      else let: "x" := (rand("α") #1) in
            if: ("x" < #1)
            then "f" ("n" - #1) "α"
            else "f" ("n" + #1) "α")%V.
@@ -26,25 +26,57 @@ Section uniform_random_walk.
     ( let: "α" := (alloc #1) in
       unif_rw_1d_rec #1 "α" )%E.
 
-  Fixpoint final_pos_rev (p0 : nat) (li : list (fin 2)) : nat :=
+  Fixpoint final_pos (p0 : nat) (li : list (fin 2)) : nat :=
     match li with
       | [] => p0
       | (x::xs) =>
-          match (final_pos_rev p0 xs) with
+          match p0 with
           | 0 => 0
           | S n => if (bool_decide (x = 0%fin))
-                     then n
-                     else (S (S n))
+                     then final_pos n xs
+                     else final_pos (S (S n)) xs
           end
     end.
 
-  Definition final_pos (p0 : nat) (li : list (fin 2)) : nat :=
-    final_pos_rev p0 (reverse li).
+  Lemma final_pos_app (p0 : nat) (li : list (fin 2)) (i : fin 2) :
+    final_pos p0 (li ++ [i]) =
+      match final_pos p0 li with
+        | 0 => 0%nat
+        | S n =>
+            if (bool_decide (i = 0%fin))
+                then n
+                else (S (S n))
+       end.
+  Proof.
+    revert p0.
+    induction li; intro p0.
+    - simpl. done.
+    - rewrite -app_comm_cons.
+      simpl.
+      destruct p0; auto.
+      destruct (decide (a = 0%fin)).
+      + rewrite (bool_decide_eq_true_2 (a = 0%fin)); auto.
+      + rewrite (bool_decide_eq_false_2 (a = 0%fin)); auto.
+  Qed.
+
+
 
   Definition final_pos_rsm (p0 : nat) (li : list (fin 2)) : R :=
-    final_pos_rev p0 (reverse li).
+    final_pos p0 li.
 
   Definition term_cond (p0 : nat) (li : list (fin 2)) := (final_pos p0 li = 0%nat).
+
+  Lemma term_cond_0 (p0 : nat) (li : list (fin 2)) :
+    term_cond (S p0) (0%fin :: li) <-> term_cond p0 li.
+  Proof.
+    rewrite /term_cond; simpl; auto.
+  Qed.
+
+  Lemma term_cond_1 (p0 : nat) (li : list (fin 2)) :
+    term_cond (S p0) (1%fin :: li) <-> term_cond (S (S p0)) li.
+  Proof.
+    rewrite /term_cond; simpl; auto.
+  Qed.
 
   Lemma final_pos_rsm_pos (li : list (fin 2)) :
     0 <= final_pos_rsm 1 li.
@@ -52,19 +84,51 @@ Section uniform_random_walk.
     apply pos_INR.
   Qed.
 
+  Lemma final_pos_dec_aux (p0 : nat) (li : list (fin 2)):
+    ¬ term_cond p0 li → final_pos p0 (li ++ [0%fin]) < final_pos p0 li.
+  Proof.
+    revert p0.
+    induction li; intro p0.
+    - rewrite /term_cond.
+      intros Hterm.
+      simpl.
+      destruct p0.
+      + rewrite /final_pos // in Hterm.
+      + apply lt_INR.
+        lia.
+    - intros Hterm.
+      rewrite -app_comm_cons.
+      simpl.
+      destruct p0.
+      + rewrite /term_cond /final_pos // in Hterm.
+      + case_bool_decide.
+        * apply IHli.
+          intros Htc.
+          apply Hterm.
+          simplify_eq.
+          rewrite term_cond_0 //.
+        * apply IHli.
+          intros Htc.
+          apply Hterm.
+          simplify_eq.
+          assert (a = 1%fin) as ->.
+          {
+            inv_fin a; auto.
+            - intros ? ?. done.
+            - intros i ? ?.
+              inv_fin i.
+              + intros ??. done.
+              + done.}
+          rewrite term_cond_1 //.
+  Qed.
+
+
   Lemma final_pos_dec (li : list (fin 2)):
         ¬ term_cond 1 li → ∃ c : fin 2, final_pos 1 (li ++ [c]) < final_pos 1 li.
   Proof.
-    rewrite /term_cond.
-    intros Hli.
+    intros H.
     exists 0%fin.
-    rewrite /final_pos.
-    rewrite /final_pos in Hli.
-    rewrite reverse_app reverse_singleton //.
-    simpl.
-    destruct (final_pos_rev 1 (reverse li)); [done|].
-    apply lt_INR.
-    lia.
+    by apply final_pos_dec_aux.
   Qed.
 
   Lemma final_pos_bounded_rsm (r : R):
@@ -92,47 +156,92 @@ Section uniform_random_walk.
   Proof.
     rewrite SeriesC_fin2.
     rewrite /final_pos_rsm.
-    do 2 rewrite reverse_app reverse_singleton //.
-    simpl.
-    destruct (final_pos_rev 1 (reverse l)); [lra|].
+    do 2 rewrite final_pos_app.
+    destruct (final_pos 1 l); [lra|].
+    case_bool_decide; [|done].
+    case_bool_decide; [done|].
     do 2 rewrite S_INR.
     lra.
   Qed.
 
   Theorem rw_final_pos (n : nat) (li : list (fin 2)) (α : loc) E :
     term_cond n li ->
-    α ↪ (1%nat; li) -∗
-    WP unif_rw_1d_rec #n (#lbl:α) @ E {{ v, True }}.
+    α ↪ (S (Z.to_nat 0); li) -∗
+    WP unif_rw_1d_rec #n (#lbl:α) @ E [{ v, True }].
   Proof.
     iIntros (Hterm) "Hα".
-    iInduction li as [|i lr] "IH".
+    iInduction li as [|i lr] "IH" forall (n Hterm).
     - rewrite /term_cond /final_pos /= in Hterm.
       rewrite Hterm.
       rewrite /unif_rw_1d_rec.
       wp_pures.
       done.
     - rewrite /unif_rw_1d_rec.
+      destruct n as [|m].
+      (* Corner case: n = 0 *)
+      {
+        wp_pures. done.
+      }
       wp_pures.
-      case_bool_decide.
-      + wp_pures. done.
-      + wp_pures.
-        wp_bind (rand _)%E.
-        (* TODO : Fix rand_tape tactic *)
-        iPoseProof (wp_rand_tape 1 α i lr 1 E with "[$Hα]") as "Hklj".
-  Admitted.
+      rewrite bool_decide_eq_false_2 ; [|lia].
+      wp_pures.
+      wp_bind (Rand _ _)%I.
+      (* TODO : Fix rand_tape tactic *)
+      wp_apply (twp_rand_tape with "Hα").
+      iIntros "Hα".
+      wp_pures.
+      case_bool_decide as Hi.
+      * do 2 wp_pure.
+        assert (term_cond m lr).
+        {
+          assert (i = 0%fin) as ->.
+          {
+            inv_fin i.
+            - intros ??. done.
+            - intros i ??.
+              inv_fin i.
+              + intros ??. done.
+              + intros ???.
+                simpl in Hi. lia.
+          }
+          rewrite -term_cond_0 //.
+        }
+        replace #(S m - 1) with #m; last first.
+        { do 2 f_equal. lia. }
+        iApply "IH"; auto.
+      * do 2 wp_pure.
+        assert (term_cond (S (S m)) lr).
+        {
+          assert (i = 1%fin) as ->.
+          {
+            inv_fin i.
+            - intros ??. done.
+            - intros i ??.
+              simpl in Hi.
+              inv_fin i.
+              + intros ??. done.
+              + intros i ??.
+                inv_fin i.
+          }
+          rewrite -term_cond_0 //.
+        }
+        replace #(S m + 1) with #(S (S m)); last first.
+        { do 2 f_equal. lia. }
+        iApply "IH"; auto.
+  Qed.
 
-  Theorem unif_rw_1d_AST (n : nat) (ε : nonnegreal) E :
+  Theorem unif_rw_1d_AST (ε : nonnegreal) E :
     (0 < ε)%R ->
     ↯ ε -∗
-           WP unif_rw_1d @ E {{ v, True }}.
+           WP unif_rw_1d @ E [{ v, ⌜ True ⌝ }].
   Proof.
     iIntros (Hpos) "Herr".
     rewrite /unif_rw_1d.
     (* TODO: fix wp_alloctape tactic *)
-    wp_apply (wp_alloc_tape); auto.
+    wp_apply (twp_alloc_tape); auto.
     iIntros (α) "Hα".
     do 2 wp_pure.
-    wp_apply (presample_rsm 1 1 _ _ _ _ (term_cond 1) _ _ (final_pos_rsm 1) (final_pos 1)); eauto.
+    wp_apply (twp_presample_rsm 1 1 _ _ _ _ (term_cond 1) _ _ (final_pos_rsm 1) (final_pos 1)); eauto.
     - apply final_pos_rsm_pos.
     - intros l.
       rewrite /term_cond /final_pos_rsm /final_pos //.
@@ -149,3 +258,22 @@ Section uniform_random_walk.
   Qed.
 
 End uniform_random_walk.
+
+Theorem unif_rw_1d_AST_external Σ `{erisGpreS Σ} (σ : state) :
+  (SeriesC (lim_exec (unif_rw_1d, σ)) = 1)%R.
+Proof.
+  assert (1 - 0 <= SeriesC (lim_exec (unif_rw_1d, σ)))%R as Haux; last first.
+  {
+    rewrite Rminus_0_r in Haux.
+    apply Rle_antisym; auto.
+  }
+  eapply (twp_mass_lim_exec_limit _ _ _ _ (fun _ => True)); [lra|].
+  intros ? ε Hε.
+  iStartProof.
+  iIntros "Herr".
+  iPoseProof (ec_eq _ (nonneg (mknonnegreal _ (Rlt_le _ _ Hε))) with "Herr") as "Herr";
+    [simpl;done|].
+  iApply (unif_rw_1d_AST with "Herr").
+  simpl; lra.
+Qed.
+
